src/program_proof/tulip/res_group.v
@@ -7,6 +7,7 @@ Section res.
   (* TODO: remove this once we have real defintions for resources. *)
   Implicit Type (γ : tulip_names).
 
+  (* TODO: rename this to [group_prepare]. *)
   Section group_prep.
 
     (** Mapping from transaction IDs to preparedness of transactions on a group. *)
@@ -53,5 +54,52 @@ Section res.
     Admitted.
 
   End group_prep.
+
+  Section group_commit.
+
+    (** Mapping from transaction IDs to committedness of transactions on a group. *)
+
+    Definition own_group_commit_map γ (gid : u64) (pm : gmap nat bool) : iProp Σ.
+    Admitted.
+
+    Definition is_group_commit γ (gid : u64) (ts : nat) (c : bool) : iProp Σ.
+    Admitted.
+
+    #[global]
+    Instance is_group_commit_persistent γ gid ts c :
+      Persistent (is_group_commit γ gid ts c).
+    Admitted.
+
+    Definition is_group_committed γ gid ts :=
+      is_group_commit γ gid ts true.
+
+    Definition is_group_aborted γ gid ts :=
+      is_group_commit γ gid ts false.
+
+    Lemma group_commit_agree γ gid ts c1 c2 :
+      is_group_commit γ gid ts c1 -∗
+      is_group_commit γ gid ts c2 -∗
+      ⌜c2 = c1⌝.
+    Admitted.
+
+    Lemma group_commit_insert {γ gid pm} ts c :
+      pm !! ts = None ->
+      own_group_commit_map γ gid pm ==∗
+      own_group_commit_map γ gid (<[ts := c]> pm) ∗ is_group_commit γ gid ts c.
+    Admitted.
+
+    Lemma group_commit_witness γ gid pm ts c :
+      pm !! ts = Some c ->
+      own_group_commit_map γ gid pm -∗
+      is_group_commit γ gid ts c.
+    Admitted.
+
+    Lemma group_commit_lookup γ gid pm ts c :
+      own_group_commit_map γ gid pm -∗
+      is_group_commit γ gid ts c -∗
+      ⌜pm !! ts = Some c⌝.
+    Admitted.
+
+  End group_commit.
 
 End res.
