src/program_proof/rsm/pure/nat.v
@@ -9,6 +9,16 @@ Definition le_all (n : nat) (ns : gset nat) :=
 Definition gt_all (n : nat) (ns : gset nat) :=
   set_Forall (λ x, x < n)%nat ns.
 
+Lemma gt_all_weaken {ns n} n' :
+  (n ≤ n')%nat ->
+  gt_all n ns ->
+  gt_all n' ns.
+Proof.
+  intros Hge Hgtall x Hx.
+  specialize (Hgtall _ Hx). simpl in Hgtall.
+  lia.
+Qed.
+
 Definition ge_all (n : nat) (ns : gset nat) :=
   set_Forall (λ x, x ≤ n)%nat ns.
 
@@ -17,3 +27,23 @@ Definition nz_all (ns : gset nat) :=
 
 Definition outside_all (ub lb : nat) (ns : gset nat) :=
   set_Forall (λ x, x ≤ ub ∨ lb < x)%nat ns.
+
+Lemma outside_all_weaken_ub {ns ub lb} ub' :
+  (ub ≤ ub')%nat ->
+  outside_all ub lb ns ->
+  outside_all ub' lb ns.
+Proof.
+  intros Hle Houtside n Hn.
+  specialize (Houtside _ Hn).
+  destruct Houtside; lia.
+Qed.
+
+Lemma outside_all_weaken_lb {ns ub lb} lb' :
+  (lb' ≤ lb)%nat ->
+  outside_all ub lb ns ->
+  outside_all ub lb' ns.
+Proof.
+  intros Hge Houtside n Hn.
+  specialize (Houtside _ Hn).
+  destruct Houtside; lia.
+Qed.
